@prefix : <http://bim.aalto.fi/DiCtion/Ontology/> .
@prefix owl: <http://www.w3.org/2002/07/owl#> .
@prefix rdf: <http://www.w3.org/1999/02/22-rdf-syntax-ns#> .
@prefix xml: <http://www.w3.org/XML/1998/namespace> .
@prefix xsd: <http://www.w3.org/2001/XMLSchema#> .
@prefix rdfs: <http://www.w3.org/2000/01/rdf-schema#> .
@base <http://bim.aalto.fi/DiCtion/Ontology/> .

<http://bim.aalto.fi/DiCtion/Ontology/> rdf:type owl:Ontology ;
                                         owl:versionIRI <http://bim.aalto.fi/DiCtion/Ontology/ConstructionPlanning/0.9.1> ;
                                         <http://purl.org/dc/terms/creator> "Seppo Torma"@en ,
                                                                            "Yuan Zheng"@en ;
                                         rdfs:comment "The construction planning ontology is one module of DiCtion Shared Situation Awareness ontology that refers the collection of concepts and relationships that are relevant with the the construction planning process. The construction planning process is activity-oriented that focus on what kind of conditions an activity has and what kinds of resource the activity is requiring."@en ;
                                         owl:versionInfo "0.9.1"@en .

#################################################################
#    Annotation properties
#################################################################

###  http://purl.org/dc/terms/creator
<http://purl.org/dc/terms/creator> rdf:type owl:AnnotationProperty .


#################################################################
#    Object Properties
#################################################################

###  http://bim.aalto.fi/DiCtion/Ontology/Precondition
:Precondition rdf:type owl:ObjectProperty ;
              rdfs:subPropertyOf :hasCondition ;
              rdfs:comment "A relation between an 'Activity' and its required initial condition of conduction."@en .


###  http://bim.aalto.fi/DiCtion/Ontology/addEffect
:addEffect rdf:type owl:ObjectProperty ;
           rdfs:subPropertyOf :hasCondition ;
           rdfs:comment "A relation that the execution of an  'Activity' will add some new conditions."@en .


###  http://bim.aalto.fi/DiCtion/Ontology/completionCondition
:completionCondition rdf:type owl:ObjectProperty ;
                     rdfs:subPropertyOf :hasCondition ;
                     rdfs:comment "A relation of an 'Activity' and its completion condition (the condition of the activity is completed)."@en .


###  http://bim.aalto.fi/DiCtion/Ontology/deleteEffect
:deleteEffect rdf:type owl:ObjectProperty ;
              rdfs:subPropertyOf :hasCondition ;
              rdfs:comment "A relation that the execution of an 'Activity' will remove some new conditions."@en .


###  http://bim.aalto.fi/DiCtion/Ontology/executionCondition
:executionCondition rdf:type owl:ObjectProperty ;
                    rdfs:subPropertyOf :hasCondition ;
                    rdfs:comment "The relation between an 'Activity' and its execution condition (the conditions that enable the activity to be executable, also known as the constraints of executing)."@en .


###  http://bim.aalto.fi/DiCtion/Ontology/hasCapability
:hasCapability rdf:type owl:ObjectProperty ;
               rdfs:domain :Resource ;
               rdfs:range :Capacity ;
               rdfs:comment "A relation between a 'Resource' and its 'Capacity'"@en .


###  http://bim.aalto.fi/DiCtion/Ontology/hasCondition
:hasCondition rdf:type owl:ObjectProperty ;
              rdfs:domain :Activity ;
              rdfs:range :Condition ;
              rdfs:comment "A relation between an 'Activity' and its conditions."@en .


###  http://bim.aalto.fi/DiCtion/Ontology/hasObject
:hasObject rdf:type owl:ObjectProperty ;
           rdfs:domain :ObjectTimeInterval ;
           rdfs:range :DomainObject ;
           rdfs:comment "A relation of between object-relevant concepts and their related domain object"@en .


###  http://bim.aalto.fi/DiCtion/Ontology/hasType
:hasType rdf:type owl:ObjectProperty ;
         rdfs:domain :Activity ,
                     :CapabilityRequirement ,
                     :ResourceTypeRequirement ;
         rdfs:range :ActivityType ,
                    :CapabilityType ,
                    :ResourceType ;
         rdfs:comment "a relations indicate an instance of a concept has correspondent type."@en .


###  http://bim.aalto.fi/DiCtion/Ontology/isDerivedfrom
:isDerivedfrom rdf:type owl:ObjectProperty ;
               rdfs:domain :Condition ;
               rdfs:range :Event ;
               rdfs:comment "A relation between 'Condition' and 'Event' that the condition information is derived from related event records."@en .


###  http://bim.aalto.fi/DiCtion/Ontology/precedes
:precedes rdf:type owl:ObjectProperty ;
          rdfs:domain :Activity ;
          rdfs:range :Activity ;
          rdfs:comment "The squential relationship between an activity and its succesor activity" .


###  http://bim.aalto.fi/DiCtion/Ontology/requires
:requires rdf:type owl:ObjectProperty ;
          rdfs:domain :Activity ;
          rdfs:range :Requirement ;
          rdfs:comment "A relation between a 'Activity' and 'Requirement' that activity requires some requirements" .


#################################################################
#    Data properties
#################################################################

###  http://bim.aalto.fi/DiCtion/Ontology/hasRequiredAmount
:hasRequiredAmount rdf:type owl:DatatypeProperty ;
                   rdfs:domain :Requirement ;
                   rdfs:comment "a relation between quantity-relevant requirements and their required quantity" .


###  http://bim.aalto.fi/DiCtion/Ontology/hasUnit
:hasUnit rdf:type owl:DatatypeProperty ;
         rdfs:domain :Requirement ,
                     :Resource ;
         rdfs:comment "a relation between quantity-relevant concepts and their unit" .


###  http://bim.aalto.fi/DiCtion/Ontology/hasWorkRate
:hasWorkRate rdf:type owl:DatatypeProperty ;
             rdfs:domain :Capacity ;
             rdfs:comment "a relation between capacity and their numerical work-rate" .


#################################################################
#    Classes
#################################################################

###  http://bim.aalto.fi/DiCtion/Ontology/Activity
:Activity rdf:type owl:Class ;
          rdfs:subClassOf :DomainObject ,
                          :ObjectTimeInterval ,
                          [ rdf:type owl:Restriction ;
                            owl:onProperty :hasType ;
                            owl:allValuesFrom :ActivityType
                          ] ;
          rdfs:comment "Activity is the concept refers to all the works (or aggregations of works) that carried out in a construction project."@en .


###  http://bim.aalto.fi/DiCtion/Ontology/ActivityType
:ActivityType rdf:type owl:Class ;
              rdfs:comment "The type of the activity"@en .


###  http://bim.aalto.fi/DiCtion/Ontology/CapabilityRequirement
:CapabilityRequirement rdf:type owl:Class ;
                       rdfs:subClassOf :Requirement ,
                                       [ rdf:type owl:Restriction ;
                                         owl:onProperty :hasType ;
                                         owl:allValuesFrom :CapabilityType
                                       ] ;
                       rdfs:comment "Capability requirement refers that an activity requires the resource should have specific capability."@en .


###  http://bim.aalto.fi/DiCtion/Ontology/CapabilityType
:CapabilityType rdf:type owl:Class ;
                rdfs:comment "The type of the capability that the resource has"@en .


###  http://bim.aalto.fi/DiCtion/Ontology/Capacity
:Capacity rdf:type owl:Class ;
          rdfs:comment "Capacity concept refers to the maxium amount of a resource or material that is provided to the construction site."@en .


###  http://bim.aalto.fi/DiCtion/Ontology/Condition
:Condition rdf:type owl:Class ;
           rdfs:subClassOf :ObjectTimeInterval ;
           rdfs:comment "Condition is a concept to capture a semantically meaningful state of an object, such as its location or temperature at a level that is needed for construction management."@en .


###  http://bim.aalto.fi/DiCtion/Ontology/DomainObject
:DomainObject rdf:type owl:Class ;
              rdfs:comment "Domain objects is a abstract concept that refers to all the central objects that are discussed in the construction project planning and management. Sub-classes of the domain object include the 'Activity','Group','Information Entity','Physical Entity',and 'Resource'."@en .


###  http://bim.aalto.fi/DiCtion/Ontology/Event
:Event rdf:type owl:Class ;
       rdfs:subClassOf :InformationEntity .


###  http://bim.aalto.fi/DiCtion/Ontology/InformationEntity
:InformationEntity rdf:type owl:Class ;
                   rdfs:subClassOf :DomainObject .


###  http://bim.aalto.fi/DiCtion/Ontology/ObjectTimeInterval
:ObjectTimeInterval rdf:type owl:Class ;
                    rdfs:subClassOf <http://www.w3.org/2006/time#Interval> ;
                    rdfs:comment "A temporal entity with an extent or duration that has related domain object."@en .


###  http://bim.aalto.fi/DiCtion/Ontology/Requirement
:Requirement rdf:type owl:Class ;
             rdfs:comment "The requirement concept refers to the request of the resource for one activity, which including capability requirement and the resource type requirement of the resource."@en .


###  http://bim.aalto.fi/DiCtion/Ontology/Resource
:Resource rdf:type owl:Class ;
          rdfs:subClassOf :DomainObject .


###  http://bim.aalto.fi/DiCtion/Ontology/ResourceType
:ResourceType rdf:type owl:Class ;
              rdfs:comment "The type of the resource"@en .


###  http://bim.aalto.fi/DiCtion/Ontology/ResourceTypeRequirement
:ResourceTypeRequirement rdf:type owl:Class ;
                         rdfs:subClassOf :Requirement ,
                                         [ rdf:type owl:Restriction ;
                                           owl:onProperty :hasType ;
                                           owl:allValuesFrom :ResourceType
                                         ] ;
                         rdfs:comment "Resource Type requirement refers that an activity requires the resource should have specific type."@en .


###  http://www.w3.org/2006/time#Interval
<http://www.w3.org/2006/time#Interval> rdf:type owl:Class .


###  Generated by the OWL API (version 5.1.7) https://github.com/owlcs/owlapi/
